doc/strtoimax/Core/IntLemmas.v
@@ -1,0 +1,416 @@
+Require Import StructTact.StructTactics.
+Require Import Core Notations.
+
+
+(** * Some lemmas about integers *)
+
+Definition IntMax := Int.repr Int.max_unsigned.
+
+Lemma int_to_unsigned_eq : forall i j, i = j <-> Int.unsigned i = Int.unsigned j.
+Proof.
+  intros.
+  destruct i.
+  destruct j.
+  split.
+  * congruence.
+  * apply Int.mkint_eq.
+Qed.
+
+Lemma int_to_unsigned_neq : forall i j, i <> j -> Int.unsigned i <> Int.unsigned j.
+Proof.
+  intros.
+  destruct (zeq (Int.unsigned i) (Int.unsigned j)) eqn : G.
+  pose (Int.eq_false _ _ H).
+  unfold Int.eq in e0.
+  rewrite G in e0.
+  congruence.
+  assumption.
+Qed.
+
+Lemma non_zero_surj :
+  forall i, Int.add i Int.one <> Int.zero ->
+       Int.unsigned (Int.add i Int.one) = Int.unsigned i + 1.
+Proof.
+  intros.
+  destruct (Z.eq_dec (Int.unsigned (Int.add i Int.one)) (Int.unsigned i + 1)).
+  intuition.
+  unfold Int.add in n.
+  assert (i <> IntMax).
+  destruct (Int.eq_dec i IntMax).
+  rewrite e in H.
+  
+  assert (Int.add IntMax Int.one = Int.zero).
+  { unfold IntMax.
+    unfold Int.add.
+    unfold Int.zero.
+    simpl; unfold Int.add; unfold Int.mul;
+      repeat rewrite Int.unsigned_repr_eq;
+      repeat rewrite Int.unsigned_repr_eq;
+      repeat rewrite Zmod_small.
+    replace (Int.max_unsigned + Int.unsigned Int.one) with (Int.modulus) by (auto with ints).
+    pose (Int.mkint_eq).
+    destruct  (Int.repr Int.modulus) eqn : IM.
+    destruct (Int.repr 0) eqn : S0.
+    apply Int.mkint_eq.
+    assert (Int.repr Int.modulus =
+            Int.mkint (Int.Z_mod_modulus Int.modulus) (Int.Z_mod_modulus_range' Int.modulus))
+      by (auto with ints).
+    rewrite H0 in IM.
+    inversion IM.
+    inversion S0.
+    replace (match Int.repr 0 with
+             | {| Int.intval := intval1 |} => intval1
+             end) with 0 by (auto with ints).
+    auto.
+    cbv.
+    split; congruence.
+  }
+  congruence.
+  assumption.
+  simpl; unfold Int.add; unfold Int.mul;
+    repeat rewrite Int.unsigned_repr_eq;
+    repeat rewrite Int.unsigned_repr_eq;
+    repeat rewrite Zmod_small.
+  auto with ints.
+  assert (Int.unsigned i < Int.max_unsigned).
+  assert (Int.unsigned i <> Int.unsigned IntMax) by (eapply (int_to_unsigned_neq _ _ H0)).
+  destruct i; simpl in *.
+  unfold IntMax in *.
+  replace (Int.unsigned (Int.repr Int.max_unsigned)) with (Int.max_unsigned) in H1 by (auto with ints).
+  unfold Int.max_unsigned in *.
+  nia.
+  unfold Int.max_unsigned in *.
+  replace (Int.unsigned Int.one) with 1 by (auto with ints). 
+  pose (Int.unsigned_range i).
+  nia.
+Qed.
+
+Lemma int_overflow_unsigned_to_add :
+  forall z, 0 < Int.unsigned z + 1 < Int.modulus ->
+       Int.add z Int.one <> Int.zero.
+Proof.
+  intros.
+  unfold Int.zero.
+  destruct (Int.eq (Int.add z Int.one) (Int.repr 0)) eqn: Sz.
+  pose (Int.eq_spec (Int.add z Int.one) (Int.repr 0)) as E.
+  unfold Int.eq in Sz.
+  destruct (zeq (Int.unsigned (Int.add z Int.one))
+                (Int.unsigned (Int.repr 0))).
+  unfold Int.add in e.
+  repeat rewrite Int.unsigned_repr_eq in e.
+  rewrite Zmod_small in e.
+  rewrite  Zmod_small in e.
+  replace (Int.unsigned Int.one) with 1 in e by (auto with ints).  nia.
+  nia.
+  replace (Int.unsigned Int.one) with 1 by (auto with ints).  nia.
+  congruence.
+  pose (Int.eq_spec (Int.add z Int.one)  (Int.repr 0)).
+  rewrite Sz in y.
+  assumption. 
+Qed.
+
+(* Induction principle for integers *)
+
+Lemma int_induction :
+  forall (P : int -> Prop),
+    P Int.zero ->
+    (forall i, P i -> P (Int.add i Int.one))
+    -> forall i, P i.
+Proof.
+  induction i.
+  eapply (natlike_ind (fun intval => forall intrange : -1 < intval < Int.modulus,
+                           P {| Int.intval := intval; Int.intrange := intrange |})).
+  (* Base case *)
+  - intro.
+    unfold Int.zero in H.
+    assert ((Int.repr 0) = {| Int.intval := 0; Int.intrange := intrange0 |}).
+    assert (Int.unsigned {| Int.intval := 0; Int.intrange := intrange0 |} =
+            Int.unsigned (Int.repr (0))).
+    { simpl.
+      rewrite Int.unsigned_repr.
+      auto.
+      unfold Int.max_unsigned.
+      nia. }    
+    destruct (Int.repr 0) eqn: S0.
+    apply Int.mkint_eq.
+    simpl in H1.
+    nia.
+    rewrite  H1 in H.
+    assumption.
+  - intros.
+    assert (X: -1 < x < Int.modulus) by nia.
+    pose (p := H2 X).
+    pose (H0 {| Int.intval := x; Int.intrange := X |} p).
+    assert ({| Int.intval := Z.succ x; Int.intrange := intrange0 |} =
+            (Int.add {| Int.intval := x; Int.intrange := X |} Int.one)).
+    unfold Int.add.
+    unfold Int.one.
+    unfold Int.unsigned.
+    replace (Int.intval (Int.repr 1)) with 1 by (auto with ints).
+    simpl.
+    replace (x + 1) with (Z.succ x) by nia.
+    assert (Int.unsigned {| Int.intval := Z.succ x; Int.intrange := intrange0 |} =
+            Int.unsigned (Int.repr (Z.succ x))).
+    simpl.
+    rewrite Int.unsigned_repr.
+    auto.
+    unfold Int.max_unsigned.
+    nia.
+    destruct (Int.repr (Z.succ x)) eqn: Sa.
+    apply Int.mkint_eq.
+    simpl in H3.
+    assumption.
+    rewrite <- H3 in p0.
+    assumption.
+  - nia.
+Qed.
+
+Lemma intval_eq : forall (n i : int),
+    match n with | {| Int.intval := intval |} => intval end =
+    match i with | {| Int.intval := intval |} => intval end ->
+    (n = i).
+Proof.
+  intros.
+  destruct (n) eqn: Sn.
+  destruct (i) eqn: Si. 
+  apply Int.mkint_eq.
+  assumption.
+Qed.
+  
+Lemma int_le_trans : forall a b c,
+    (a <= b)%int = true ->
+    (b <= c)%int = true ->
+    (a <= c)%int = true.
+Proof.
+  intros.
+  unfold Int.lt in *.
+  repeat break_match.
+  all: try discriminate.
+  lia.
+  reflexivity.
+Qed.
+
+Lemma int_lt_trans : forall a b c,
+    (a < b)%int = true ->
+    (b < c)%int = true ->
+    (a < c)%int = true.
+Proof.
+  intros.
+  unfold Int.lt in *.
+  repeat break_match.
+  all: try discriminate.
+  reflexivity.
+  lia.
+Qed.
+
+Lemma int64_lt_trans : forall a b c,
+    (a < b)%int64 = true ->
+    (b < c)%int64 = true ->
+    (a < c)%int64 = true.
+Proof.
+  intros.
+  unfold Int64.lt in *.
+  repeat break_match.
+  all: try discriminate.
+  reflexivity.
+  lia.
+Qed.
+
+Lemma int64_le_trans : forall a b c,
+    (a <= b)%int64 = true ->
+    (b <= c)%int64 = true ->
+    (a <= c)%int64 = true.
+Proof.
+  intros.
+  unfold Int64.lt, negb in *.
+  repeat break_match.
+  all: try discriminate.
+  lia.
+  reflexivity.
+Qed.
+
+Lemma int_le_signed_le : forall a b,
+  (a <= b)%int = true <->
+  Int.signed a <= Int.signed b.
+Proof.
+  split; intros.
+  - unfold Int.lt in H.
+    destruct zlt; [discriminate | lia].
+  - unfold Int.lt.
+    destruct zlt; [lia | reflexivity].
+Qed.
+
+Lemma int_lt_signed_lt : forall a b,
+  (a < b)%int = true <->
+  Int.signed a < Int.signed b.
+Proof.
+  split; intros.
+  - unfold Int.lt in H.
+    destruct zlt; [lia | discriminate].
+  - unfold Int.lt.
+    destruct zlt; [reflexivity | lia].
+Qed.
+
+Lemma sem_Cle_Cge : forall i a b m is1 is2,
+  sem_cmp Cge (Vint a) (Tint is1 Signed noattr)
+              (Vint b) (Tint is2 Signed noattr) m
+  = Some (Val.of_bool i)
+  <->
+  sem_cmp Cle (Vint b) (Tint is2 Signed noattr)
+              (Vint a) (Tint is1 Signed noattr) m
+  = Some (Val.of_bool i).
+Proof.
+  unfold sem_cmp, sem_binarith, sem_cast,
+         classify_cmp, classify_cast, binarith_type;
+    simpl.
+  destruct is1, is2; simpl.
+  all: destruct Archi.ptr64; simpl.
+  all: unfold Val.of_bool.
+  all: split; intros.
+  all: repeat break_match.
+  all: try reflexivity.
+  all: try discriminate.
+Qed.
+
+Lemma int_le_sem_Cle : forall i a b m is1 is2,
+  (a <= b)%int = i <->
+  sem_cmp Cle (Vint a) (Tint is1 Signed noattr)
+              (Vint b) (Tint is2 Signed noattr) m
+  = Some (Val.of_bool i).
+Proof.
+  destruct i.
+  - unfold sem_cmp, sem_binarith, sem_cast, classify_cmp; simpl.
+    split; intros.
+    -- all: destruct is1, is2; simpl.
+       all: destruct Archi.ptr64; simpl.
+       all: rewrite H; reflexivity.
+    -- all: destruct is1, is2; simpl.
+       all: unfold classify_cast, binarith_type in H.
+       all: destruct Archi.ptr64; simpl in H.
+       all: unfold Val.of_bool in H.
+       all: break_match.
+       all: try discriminate.
+       all: try reflexivity.
+  - unfold sem_cmp, sem_binarith, sem_cast, classify_cmp; simpl.
+    split; intros.
+    -- all: destruct is1, is2; simpl.
+       all: destruct Archi.ptr64; simpl.
+       all: rewrite H; reflexivity.
+    -- all: destruct is1, is2; simpl.
+       all: unfold classify_cast, binarith_type in H.
+       all: destruct Archi.ptr64; simpl in H.
+       all: unfold Val.of_bool in H.
+       all: break_match.
+       all: try discriminate.
+       all: try reflexivity.   
+Qed.
+
+Lemma int_lt_sem_Clt : forall a b m is1 is2,
+  (a < b)%int = true <->
+  sem_cmp Clt (Vint a) (Tint is1 Signed noattr)
+              (Vint b) (Tint is2 Signed noattr) m
+  = Some Vtrue.
+Proof.
+  unfold sem_cmp, sem_binarith, sem_cast, classify_cmp; simpl.
+  split; intros.
+  - all: destruct is1, is2; simpl.
+    all: destruct Archi.ptr64; simpl.
+    all: rewrite H; reflexivity.
+  - all: destruct is1, is2; simpl.
+    all: unfold classify_cast, binarith_type in H.
+    all: destruct Archi.ptr64; simpl in H.
+    all: unfold Val.of_bool in H.
+    all: break_match.
+    all: try discriminate.
+    all: try reflexivity.
+Qed.
+
+Lemma sem_Clt_Cge : forall a b m is1 is2,
+  sem_cmp Cge (Vint a) (Tint is1 Signed noattr)
+              (Vint b) (Tint is2 Signed noattr) m
+  = Some Vtrue
+  <->
+  sem_cmp Clt (Vint a) (Tint is1 Signed noattr)
+              (Vint b) (Tint is2 Signed noattr) m
+  = Some Vfalse.
+Proof.
+  unfold sem_cmp, sem_binarith, sem_cast,
+         classify_cmp, classify_cast, binarith_type;
+    simpl.
+  destruct is1, is2; simpl.
+  all: destruct Archi.ptr64; simpl.
+  all: unfold Val.of_bool.
+  all: split; intros.
+  all: repeat break_match.
+  all: try reflexivity.
+  all: try discriminate.
+Qed.
+
+ 
+Lemma sem_Cle_Cgt : forall a b m is1 is2,
+  sem_cmp Cgt (Vint a) (Tint is1 Signed noattr)
+              (Vint b) (Tint is2 Signed noattr) m
+  = Some Vtrue
+  <->
+  sem_cmp Cle (Vint a) (Tint is1 Signed noattr)
+              (Vint b) (Tint is2 Signed noattr) m
+  = Some Vfalse.
+Proof.
+  unfold sem_cmp, sem_binarith, sem_cast,
+         classify_cmp, classify_cast, binarith_type;
+    simpl.
+  destruct is1, is2; simpl.
+  all: destruct Archi.ptr64; simpl.
+  all: unfold Val.of_bool.
+  all: split; intros.
+  all: repeat break_match.
+  all: try reflexivity.
+  all: try discriminate.
+Qed.
+
+
+Lemma sem_Clt_Cgt : forall a b m is1 is2,
+  sem_cmp Cgt (Vint a) (Tint is1 Signed noattr)
+              (Vint b) (Tint is2 Signed noattr) m
+  = Some Vtrue
+  <->
+  sem_cmp Clt (Vint b) (Tint is2 Signed noattr)
+              (Vint a) (Tint is1 Signed noattr) m
+  = Some Vtrue.
+Proof.
+  unfold sem_cmp, sem_binarith, sem_cast,
+         classify_cmp, classify_cast, binarith_type;
+    simpl.
+  destruct is1, is2; simpl.
+  all: destruct Archi.ptr64; simpl.
+  all: unfold Val.of_bool.
+  all: split; intros.
+  all: repeat break_match.
+  all: try reflexivity.
+  all: try discriminate.
+Qed.
+
+Lemma sem_cmp_Int_le_dec {is1 is2 : intsize} : forall a b m,
+  { sem_cmp Cle (Vint a) (Tint is1 Signed noattr)
+              (Vint b) (Tint is2 Signed noattr) m
+    = Some Vtrue } +
+  { sem_cmp Cle (Vint a) (Tint is1 Signed noattr)
+              (Vint b) (Tint is2 Signed noattr) m
+    = Some Vfalse }.
+Proof.
+  intros.
+  destruct (Z_lt_le_dec (Int.signed b) (Int.signed a)) as [LT | LE];
+    [right | left].
+  - apply sem_Cle_Cgt.
+    apply sem_Clt_Cgt.
+    apply int_lt_sem_Clt.
+    apply int_lt_signed_lt.
+    assumption.
+  - replace Vtrue with (Val.of_bool true).
+      apply int_le_sem_Cle.
+    apply int_le_signed_le.
+    assumption.
+    reflexivity.
+Qed.
+
+
