doc/strtoimax/Core/IntPtrLemmas.v
@@ -1,0 +1,422 @@
+Require Import StructTact.StructTactics.
+Require Import Core Notations Tactics IntLemmas PtrLemmas.
+
+Proposition addr_ge_to_sem_cmp_lt : forall b m b1 b2 i1 i2,
+    addr_ge m (b1, i1) (b2, i2) = Some b ->
+    sem_cmp Clt (Vptr b1 i1) (tptr tschar) (Vptr b2 i2) (tptr tschar) m = 
+    Some (Val.of_bool (negb b)).
+Proof.
+  intros.
+  eapply sem_Clt_Cge_ptr.
+  eapply ptr_ge_to_sem_cmp;
+    eassumption.
+Qed.
+
+
+Proposition distance_to_sem_cmp_lt : forall dist m b1 b2 i1 i2,
+    distance m (b1, i1) (b2, i2) = Some (S dist) ->
+    sem_cmp Clt (Vptr b1 i1) (tptr tschar)
+            (Vptr b2 i2) (tptr tschar) m = Some Vtrue.
+Proof.
+  intros until i2; intro Dist.
+  replace b1 with b2 in *.
+  pose proof (dist_to_lt _ _ _ _ _ Dist) as LT.
+  unfold distance, sem_cmp, cmp_ptr, addr_ge, ptr_ge,
+  Val.cmplu_bool, Val.cmpu_bool, Ptrofs.cmpu,
+  Val.cmp_different_blocks,
+  classify_cmp in *.
+  repeat break_match;
+    try congruence; repeat destruct_andb_hyp;
+      try congruence.
+  all: try rewrite <- ptrofs_lt_signed_lt in LT;
+    try bool_rewrite; try intuition.
+  unfold sem_binarith.
+  all: repeat break_match; simpl in *; try congruence.
+  
+  simpl in *.
+  all: unfold classify_cmp in *.
+
+  unfold distance, sem_cmp, cmp_ptr, addr_ge, ptr_ge,
+  Val.cmplu_bool, Val.cmpu_bool, Ptrofs.cmpu,
+  Val.cmp_different_blocks,
+  classify_cmp in *.
+  repeat break_match;
+    try congruence; repeat destruct_andb_hyp;
+      try congruence.
+Qed.
+
+Lemma dist_succ : forall m b b' ofs ofs' dist,
+    distance m (b', ofs') (b, ofs) = Some (S dist) ->
+    Mem.weak_valid_pointer m b' (Ptrofs.unsigned (ofs' + 1)%ptrofs) = true -> 
+    distance m (b', (Ptrofs.add ofs' Ptrofs.one)) (b, ofs) = Some dist.
+Proof.
+  unfold distance, snd; intros.
+  break_match_hyp; [| discriminate].
+  break_if; subst; [| discriminate].
+  inversion H; clear H.
+  assert (Ptrofs.unsigned ofs' < Ptrofs.max_unsigned)%Z.
+  {
+    assert ((Ptrofs.unsigned ofs') < (Ptrofs.unsigned ofs))%Z.
+    {
+      assert ((Z.to_nat (Ptrofs.unsigned ofs') 
+               < 
+               Z.to_nat (Ptrofs.unsigned ofs))%nat) by lia.
+      unfold Ptrofs.unsigned in *.
+      destruct ofs, ofs'; simpl in *.
+      pose proof (Z2Nat.inj_lt intval0 intval) as Inj.
+      destruct Inj.
+      all: try lia.
+    }
+    assert (Ptrofs.unsigned ofs <= Ptrofs.max_unsigned)%Z.
+    pose proof (Ptrofs.unsigned_range_2 ofs).
+    all: try lia.
+  }
+  replace (addr_ge m (b, ofs) (b', (ofs' + 1)%ptrofs))
+    with (Some true).
+  f_equal.
+  enough (S (Z.to_nat (Ptrofs.unsigned (ofs')%ptrofs)) =
+             Z.to_nat (Ptrofs.unsigned (ofs' + 1)%ptrofs)) by lia.
+  rewrite Ptrofs.add_unsigned, Ptrofs.unsigned_repr, <-Z2Nat.inj_succ.
+  reflexivity.
+  apply Ptrofs.unsigned_range.
+  replace (Ptrofs.unsigned 1%ptrofs) with 1 by reflexivity.
+  pose proof Ptrofs.unsigned_range ofs'.
+  lia.
+
+  unfold addr_ge, ptr_ge in *.
+  simpl in *.
+  repeat break_if; subst.
+  all: try discriminate; unfold Mem.weak_valid_pointer in *.
+  all: repeat destruct_andb_hyp.
+  all: repeat destruct_orb_hyp.
+  all: try congruence.
+  all: clear - H H2 Heqo.
+
+  all: assert (Z.to_nat (Ptrofs.unsigned ofs') + 1 <=
+          Z.to_nat (Ptrofs.unsigned ofs))%nat
+    by lia.
+  all: unfold Ptrofs.ltu.
+  all: break_if.
+  all: rewrite Ptrofs.add_unsigned, Ptrofs.unsigned_repr in *.
+  all: replace (Ptrofs.unsigned 1%ptrofs) with 1 in * by reflexivity.
+  all: replace (1)%nat with (Z.to_nat 1)%nat in H0 by reflexivity.
+  all: rewrite <-Z2Nat.inj_add in H0.
+  all: try rewrite <-Z2Nat.inj_le in H0.
+  all: try apply Ptrofs.unsigned_range.
+  all: try reflexivity.
+  all: replace (Ptrofs.unsigned 1%ptrofs) with 1 by reflexivity.
+  all: pose proof Ptrofs.unsigned_range ofs'.
+  all: try lia.
+Qed.
+
+Proposition distance_succ_no_overflow :  forall m b b' ofs ofs' dist,
+    distance m (b', ofs') (b, ofs) = Some (S dist) ->
+    Ptrofs.unsigned (ofs' + 1)%ptrofs = Ptrofs.unsigned ofs' + 1.
+Proof.
+  intros.
+  unfold distance, snd in *; intros.
+  break_match_hyp; [| discriminate].
+  break_if; subst; [| discriminate].
+  inversion H; clear H.
+  assert (Ptrofs.unsigned ofs' < Ptrofs.max_unsigned)%Z.
+  {
+    assert ((Ptrofs.unsigned ofs') < (Ptrofs.unsigned ofs))%Z.
+    {
+      assert ((Z.to_nat (Ptrofs.unsigned ofs') 
+               < 
+               Z.to_nat (Ptrofs.unsigned ofs))%nat) by lia.
+      unfold Ptrofs.unsigned in *.
+      destruct ofs, ofs'; simpl in *.
+      pose proof (Z2Nat.inj_lt intval0 intval) as Inj.
+      destruct Inj.
+      all: try lia.
+    }
+    assert (Ptrofs.unsigned ofs <= Ptrofs.max_unsigned)%Z.
+    pose proof (Ptrofs.unsigned_range_2 ofs).
+    all: try lia.
+  }
+  
+  all: rewrite Ptrofs.add_unsigned, Ptrofs.unsigned_repr in *.
+  all: replace (Ptrofs.unsigned 1%ptrofs) with 1 in * by reflexivity.
+  auto.
+  destruct ofs'; simpl in *.
+  nia.
+Qed.
+
+Proposition distance_O : forall m b1 b2 i1 i2,
+    distance m (b1,i1) (b2,i2) = Some O <->
+    ((b1,i1) = (b2,i2))%ptrofs
+    /\ Mem.weak_valid_pointer m b1 (Ptrofs.unsigned i1) = true.
+Proof.
+  intros.
+  split; unfold distance; intro.
+  -  repeat break_match; try congruence.
+     unfold addr_ge, ptr_ge,
+     Val.cmplu_bool, Val.cmpu_bool, Ptrofs.cmpu in *.
+     repeat break_match; simpl in *;
+       try congruence.
+     + inversion Heqo.
+       assert ((Ptrofs.unsigned i1) <= (Ptrofs.unsigned i2))%Z.
+       { eapply ptrofs_le_unsigned_le.
+         eassumption.
+       }
+       erewrite <- Z2Nat.inj_sub in H.
+       inversion H.
+       rewrite <- Z2Nat.inj_0 in H3.
+       assert (Ptrofs.unsigned i2 - Ptrofs.unsigned i1 = 0)%Z.
+       { eapply Z2Nat.inj.
+         all: try nia. }
+       assert (i2 = i1)%ptrofs.
+       assert (Ptrofs.unsigned i2 = Ptrofs.unsigned i1)%Z by nia.
+       apply (ptrofs_to_unsigned_eq).
+       eassumption.
+       split.
+       * f_equal.
+         symmetry; eassumption.
+         symmetry; eassumption.
+       * rewrite H1. 
+         destruct_andb_hyp. eassumption.
+       * destruct i1; simpl; nia.
+     + inversion Heqo.
+       assert ((Ptrofs.unsigned i1) <= (Ptrofs.unsigned i2))%Z.
+       { eapply ptrofs_le_unsigned_le.
+         eassumption.
+       }
+       erewrite <- Z2Nat.inj_sub in H.
+       inversion H.
+       rewrite <- Z2Nat.inj_0 in H3.
+       assert (Ptrofs.unsigned i2 - Ptrofs.unsigned i1 = 0)%Z.
+       { eapply Z2Nat.inj.
+         all: try nia. }
+       assert (i1 = i2)%ptrofs.
+       assert (Ptrofs.unsigned i1 = Ptrofs.unsigned i2)%Z by nia.
+       apply (ptrofs_to_unsigned_eq).
+       eassumption.
+       split.
+       * f_equal.
+         symmetry; eassumption.
+         eassumption.
+       * rewrite H1. 
+         destruct_andb_hyp. eassumption.
+       * destruct i1; simpl; nia.
+  - break_and.
+    inversion H.
+    rewrite <- H3.
+    rewrite <- H2.
+    repeat break_match.
+    f_equal.
+    nia.
+    repeat break_match; try congruence.
+    unfold addr_ge, ptr_ge,
+    Val.cmplu_bool, Val.cmpu_bool, Ptrofs.cmpu,
+    Ptrofs.ltu in *.
+    repeat break_match; simpl in *;
+      try congruence.
+    all: try nia.
+    
+    repeat break_match; try congruence.
+    unfold addr_ge, ptr_ge,
+    Val.cmplu_bool, Val.cmpu_bool, Ptrofs.cmpu,
+    Ptrofs.ltu in *.
+    repeat break_match; simpl in *;
+      try congruence.
+    
+    all: destruct_andb_hyp; try intuition.
+    all:unfold Mem.weak_valid_pointer in *;
+      congruence.
+Qed.
+
+Lemma dist_succ_load : forall dist c m b ofs b' ofs' v,
+    Mem.loadv c m (Vptr b' ofs') = Some v ->
+    distance m (b', ofs') (b, ofs) = Some (S dist) ->
+    distance m (b', (Ptrofs.add ofs' Ptrofs.one)) (b, ofs) = Some dist.
+Proof.
+  intros until v;
+    intros Load Dist.
+  eapply loaded_is_valid in Load.
+  eapply dist_succ.
+  eassumption.
+  unfold Mem.weak_valid_pointer.
+  replace (Ptrofs.unsigned (ofs' + 1)%ptrofs - 1)%Z with
+      (Ptrofs.unsigned ofs')%Z.
+  rewrite Load.
+  intuition.
+  eapply distance_succ_no_overflow in Dist.
+  rewrite Dist.
+  nia.
+Qed.
+
+Proposition addr_lt_ge_eq : forall b m b1 b2 i1 i2 ,
+    addr_ge m (b1, i1) (b2, i2) = Some b
+    <-> addr_lt m (b1, i1) (b2, i2) = Some (negb b).
+Proof.
+  intros.
+  unfold addr_lt.
+  simpl.
+  destruct b.
+  * unfold option_map.
+    break_match.
+    destruct b.
+    all: try (intuition || congruence).
+    all: try congruence.
+  * unfold option_map.
+    break_match.
+    destruct b.
+    all: try (intuition || congruence).
+    all: try congruence.  
+Qed.
+
+Proposition addr_lt_ge_eq' : forall b m b1 b2 i1 i2 ,
+    addr_lt m (b1, i1) (b2, i2) = Some b
+    <-> addr_ge m (b1, i1) (b2, i2) = Some (negb b).
+Proof.
+  intros.
+  unfold addr_lt.
+  simpl.
+  destruct b.
+  * unfold option_map.
+    break_match.
+    destruct b.
+    all: try (intuition || congruence).
+    all: try congruence.
+  * unfold option_map.
+    break_match.
+    destruct b.
+    all: try (intuition || congruence).
+    all: try congruence.  
+Qed.
+
+Proposition addr_ge_to_ge : forall b m b1 b2 i1 i2 ,
+    addr_ge m (b1, i1) (b2, i2) = Some b
+    -> (i2 <=u i1)%ptrofs = b.
+Proof.
+  intros.
+  unfold distance, sem_cmp, cmp_ptr, addr_lt, addr_ge, ptr_ge,
+  Val.cmplu_bool, Val.cmpu_bool, Ptrofs.cmpu,
+  Val.cmp_different_blocks,
+  classify_cmp in *.
+  repeat break_match;
+    try congruence;
+      simpl in *;
+      try congruence.
+Qed.
+
+Proposition addr_lt_to_lt : forall b m b1 b2 i1 i2 ,
+    addr_lt m (b1, i1) (b2, i2) = Some b
+    -> (i1 <u i2)%ptrofs = b.
+Proof.
+  intros.
+  unfold addr_lt in *.
+  Locate addr_lt.
+  unfold distance, sem_cmp, cmp_ptr, addr_lt, addr_ge, ptr_ge,
+  Val.cmplu_bool, Val.cmpu_bool, Ptrofs.cmpu,
+  Val.cmp_different_blocks,
+  classify_cmp in *.
+  repeat break_match;
+    try congruence;
+      simpl in *;
+      try congruence;
+      try intuition.
+  unfold Ptrofs.ltu in *.
+  repeat break_match;
+    simpl in *;
+    try congruence;
+    try nia.
+Qed.
+
+Proposition addr_lt_to_sem_cmp_lt : forall b m b1 b2 i1 i2,
+  addr_lt m (b1, i1) (b2, i2) = Some b ->
+     (sem_cmp Clt (Vptr b1 i1) (tptr tschar)
+              (Vptr b2 i2) (tptr tschar) m = Some (Val.of_bool b)).
+Proof.
+  intros until i2; intro Addr.
+  eapply sem_Clt_Cge_ptr'.
+  eapply addr_lt_ge_eq' in Addr.
+   eapply ptr_ge_to_sem_cmp;
+     eassumption.
+Qed.
+
+Proposition addr_lt_trans : forall m b1 b2 i1 i2,
+    addr_lt m (b1, (i1 + 1)%ptrofs) (b2, i2) = Some true ->
+    Ptrofs.unsigned (i1 + 1)%ptrofs = Ptrofs.unsigned i1 + 1 ->
+    Mem.weak_valid_pointer m b1 (Ptrofs.unsigned i1) = true ->
+    addr_lt m (b1, i1) (b2, i2) = Some true.
+Proof.
+  intros until i2;
+    intro Addr; intro OF;
+      intro Ptr.
+  unfold addr_lt, Mem.weak_valid_pointer in *.
+  unfold distance, sem_cmp, cmp_ptr, addr_lt, addr_ge, ptr_ge,
+  Val.cmplu_bool, Val.cmpu_bool, Ptrofs.cmpu,
+  Val.cmp_different_blocks,
+  classify_cmp in *.
+  repeat break_match;
+    try congruence;
+    simpl in *;
+    try congruence;
+    try intuition.
+  unfold Ptrofs.ltu in *.
+  repeat break_match;
+    simpl in *;
+    try congruence;
+    rewrite OF in *;
+    simpl in *;
+    try nia.
+  repeat destruct_andb_hyp;
+    repeat destruct_orb_hyp;
+    try congruence.
+  Qed.
+  
+Proposition addr_lt_succ_to_sem_cmp : forall m b1 b2 i1 i2,
+    addr_lt m (b1, (i1 + 1)%ptrofs) (b2, i2) = Some true ->
+    Ptrofs.unsigned (i1 + 1)%ptrofs = Ptrofs.unsigned i1 + 1 ->
+    Mem.weak_valid_pointer m b1 (Ptrofs.unsigned i1) = true ->
+    (sem_cmp Clt (Vptr b1 i1) (tptr tschar)
+             (Vptr b2 i2) (tptr tschar) m = Some (Val.of_bool true)).
+Proof.
+  intros until i2;
+    intro Addr; intro OF; intro Ptr.
+  eapply addr_lt_trans in Addr.
+  eapply addr_lt_to_sem_cmp_lt.
+  all: eassumption.
+Qed.
+
+Proposition mem_load_inj_ptr : forall m b1 b2 b3 i1 i2 i3,
+    Mem.load Mptr m b1 (Ptrofs.unsigned i1) = Some (Vptr b2 i2) ->
+    Mem.load Mptr m b1 (Ptrofs.unsigned i1) = Some (Vptr b3 i3) ->
+    b2 = b3 /\ i2 = i3.
+Proof.
+  intros until i3;
+    intros Mem1 Mem2.
+  split; rewrite Mem1 in Mem2;
+    inversion Mem2; auto.
+Qed.
+
+Lemma ptr_ge_is_valid : forall m b1 b2 i1 i2 ,
+  ptr_ge m b1 b2 i1 i2 = Some false ->
+  Mem.weak_valid_pointer m b1 (Ptrofs.unsigned i1) = true.
+Proof.
+  unfold Mem.weak_valid_pointer.
+  intros.
+  unfold distance, sem_cmp, cmp_ptr, addr_ge, ptr_ge,
+  Val.cmplu_bool, Val.cmpu_bool, Ptrofs.cmpu,
+  Val.cmp_different_blocks,
+  classify_cmp in *.
+  repeat break_match;
+    try congruence; repeat destruct_andb_hyp;
+      try congruence;
+      repeat destruct_orb_hyp;
+      try congruence.
+  Qed.
+
+Lemma ptrofs_le_unsigned_le_neg : forall a b,
+  (a <=u b)%ptrofs = false <->
+  not (Ptrofs.unsigned a <= Ptrofs.unsigned b)%Z.
+Proof.
+  split; intros; unfold not; intros.
+  - unfold Ptrofs.ltu in H.
+    destruct zlt; [nia | intuition].
+  - unfold Ptrofs.ltu.
+    destruct zlt; intuition.
+Qed.
+
