src/PrimitiveDecoder/ExecutableSpec.v
@@ -1,0 +1,53 @@
+Require Import Core.Core.
+Import ListNotations.
+From Coq Require Import String.
+Require Import ExtLib.Structures.Monads.
+Require Export ExtLib.Data.Monads.EitherMonad.
+Require Import ExtLib.Structures.Monad.
+
+Inductive dec_rval_error := FAIL | MORE.
+
+Record dec_rval := rval { code : dec_rval_error;
+                          consumed : Z }.
+
+Definition err T := sum dec_rval T.
+
+Instance Monad_err : Monad err := Monad_either dec_rval.
+Instance Exception_err : MonadExc dec_rval err := Exception_either dec_rval.
+
+Inductive TYPE_descriptor :=
+  def { tags : list Z;
+        elements : list TYPE_descriptor 
+      }.
+
+(* checks the tag, outputs consumed length and expected length *)
+Parameter ber_check_tag : TYPE_descriptor -> list byte -> err (Z*Z).
+
+Definition ZeroChar := Byte.repr 48.
+
+Import MonadNotation.
+Open Scope monad.
+
+(* Decoding fails : 
+   1) when calloc fails to allocate memory for the output structure sptr (FAIL) SEP spec
+   2) if ber_check_tags return FAIL (when?) or MORE (?) - executable spec
+   3) if not enough data according to length read (MORE) - executable spec
+   4) expected length doesn't fit into size (FAIL) ?
+   5) malloc buf allocation fails (FAIL) SEP spec
+ *)
+
+(* skip len bytes and add '\0' at the end *)
+Definition prim_content_decoder len ls :=
+   skipn (Z.to_nat len) 
+          ls ++ [ZeroChar].
+
+Definition prim_decoder (td : TYPE_descriptor) (ls : list byte) : err (list byte) := 
+  match ls with 
+  | [] => inl (rval FAIL 0)
+  | h :: tl => x <- ber_check_tag td ls 
+                ;; if Zlength ls - (fst x) <? (snd x)
+                   then inl (rval MORE 0)
+                   else inr (prim_content_decoder (snd x) ls)
+  end.
+
+
